@prefix : <http://www.mmdio.org/ontology/mmdio/> .
@prefix dc: <http://purl.org/dc/elements/1.1/> .
@prefix ti: <http://www.ontologydesignpatterns.org/cp/owl/timeinterval.owl#> .
@prefix c4o: <http://purl.org/spar/c4o/> .
@prefix deo: <http://purl.org/spar/deo/> .
@prefix owl: <http://www.w3.org/2002/07/owl#> .
@prefix rdf: <http://www.w3.org/1999/02/22-rdf-syntax-ns#> .
@prefix tvc: <http://purl.org/spar/tvc/> .
@prefix xml: <http://www.w3.org/XML/1998/namespace> .
@prefix xsd: <http://www.w3.org/2001/XMLSchema#> .
@prefix arco: <https://w3id.org/arco/ontology/location/> .
@prefix biro: <http://purl.org/spar/biro/> .
@prefix cito: <http://purl.org/spar/cito/> .
@prefix core: <https://w3id.org/arco/ontology/core/> .
@prefix foaf: <http://xmlns.com/foaf/0.1/> .
@prefix frbr: <http://purl.org/vocab/frbr/core#> .
@prefix memo: <https://w3id.org/irnerio/ontology/memo/> .
@prefix rdfs: <http://www.w3.org/2000/01/rdf-schema#> .
@prefix fabio: <http://purl.org/spar/fabio/2019-02-19/> .
@prefix mmdio: <http://www.mmdio.org/ontology/mmdio/> .
@prefix dcterms: <http://purl.org/dc/terms/> .
@prefix literal: <http://purl.org/spar/literal/> .
@base <http://www.mmdio.org/ontology/mmdio/> .

<https://w3id.org/irnerio-mosaico/ontology/mmdio/> rdf:type owl:Ontology ;
                                                    owl:versionIRI <https://w3id.org/irnerio-mosaico/ontology/mmdio/1.0.0> ;
                                                    rdfs:comment """### MMDIO, an OWL 2 DL ontology, provides a detailed structure to represent medieval manuscript information from diverse sources.It is built on the Memo ontology and uses the FRBR-aligned Bibliographic Ontology(FaBiO) approach to distinguish between intellectual content (Expressions) and physical forms (Manifestations). MMDIO advances this method to create a more flexible, adaptable, and interoperable system for manuscript data. By incorporating features that capture both the intellectual and physical characteristics of manuscripts, MMDIO supports a wide range of scholarly activities, from in-depth manuscript analysis to comprehensive historical research.

###The objectives of MMDIO are diverse and aim to:

1. Facilitate seamless integration and interaction between the Mosaico and Irnerio platforms, ensuring unified access to medieval manuscript data across diverse repositories, including textual content, physical characteristics, historical aspects, and artistic features, across diverse repositories.

2.  Simplify the citation complexities associated with medieval manuscripts by providing a unified data model that enables intuitive access and scholarly analysis.
3. Enhance digital archiving practices to improve the organization, retrieval, and preservation of manuscript data, facilitating efficient management and accessibility in digital libraries.

 3 .Support scholarly research by enabling complex queries that connect textual content with historical contexts, allowing scholars to trace the provenance, influence, and evolution of medieval texts.

 4.  Enhance interoperability and usability of manuscript data in the digital humanities by standardizing data representation and ensuring seamless integration across repositories.

5.  Foster interdisciplinary collaboration by promoting holistic understanding through facilitating connections among disciplines such as history, literature, and art.""" ;
                                                    rdfs:label "mmdio" .

#################################################################
#    Object Properties
#################################################################

###  http://purl.org/dc/terms/creator
dcterms:creator rdf:type owl:ObjectProperty ;
                rdfs:subPropertyOf owl:topObjectProperty ;
                rdfs:comment "Examples of a Creator include a person, an organization, or a service. Typically, the name of a Creator should be used to indicate the entity."@en-us ;
                rdfs:isDefinedBy <http://purl.org/dc/terms> ;
                rdfs:label "has creator"@en .


###  http://purl.org/dc/terms/extent
dcterms:extent rdf:type owl:ObjectProperty ;
               rdfs:range dcterms:SizeOrDuration ;
               rdfs:comment "This property indicates the extent of a resource."@en ;
               rdfs:isDefinedBy <http://purl.org/dc/terms> ;
               rdfs:label "Extent"@en-us ,
                          "has extent"@en .


###  http://purl.org/dc/terms/medium
dcterms:medium rdf:type owl:ObjectProperty ;
               rdfs:comment "This property indicates the material of a resource."@en ;
               rdfs:isDefinedBy <http://purl.org/dc/terms> ;
               rdfs:label "has medium"@en .


###  http://purl.org/spar/biro/isReferencedBy
biro:isReferencedBy rdf:type owl:ObjectProperty ;
                    rdfs:subPropertyOf owl:topObjectProperty ;
                    owl:inverseOf biro:references ;
                    rdfs:comment "The relation between a publication and the bibliographic record or bibliographic reference describing it."@en ;
                    rdfs:isDefinedBy <http://purl.org/spar/biro> ;
                    rdfs:label "is referenced by"@en .


###  http://purl.org/spar/biro/references
biro:references rdf:type owl:ObjectProperty ;
                rdfs:subPropertyOf owl:topObjectProperty ;
                rdfs:comment "The relation between a bibliographic record or a bibliographic reference and the publication being referenced."@en ;
                rdfs:isDefinedBy <http://purl.org/spar/biro> ;
                rdfs:label "references"@en .


###  http://purl.org/spar/cito/cites
cito:cites rdf:type owl:ObjectProperty ;
           owl:inverseOf cito:isCitedBy ;
           rdfs:comment "Subproperty of dcterms:relation. It refers to an entity citing a cited entity, either directly and explicitly, indirectly, or implicitly."@en ;
           rdfs:isDefinedBy <http://purl.org/spar/cito> ;
           rdfs:label "cites"@en .


###  http://purl.org/spar/cito/isCitedBy
cito:isCitedBy rdf:type owl:ObjectProperty ;
               rdfs:comment "The cited entity (the subject of the RDF triple) is cited by the citing entity (the object of the triple)."@en ,
                            "This property indicates that the cited entity is cited by the citing entity."@en ;
               rdfs:isDefinedBy <http://purl.org/spar/cito> ;
               rdfs:label "is cited by"@en .


###  http://purl.org/vocab/frbr/core#embodiment
frbr:embodiment rdf:type owl:ObjectProperty ;
                owl:inverseOf frbr:embodimentOf ;
                rdfs:comment "As defined by FRBR (http://www.ifla.org/VII/s13/frbr/frbr1.htm; http://purl.org/vocab/frbr/core#embodiment), a property representing a manifestation that embodies an expression."@en ;
                rdfs:isDefinedBy frbr: ;
                rdfs:label "has embodiment"@en .


###  http://purl.org/vocab/frbr/core#embodimentOf
frbr:embodimentOf rdf:type owl:ObjectProperty ;
                  rdfs:comment "A manifestation that embodies an expression."@en ,
                               "As defined by FRBR (http://www.ifla.org/VII/s13/frbr/frbr1.htm; http://purl.org/vocab/frbr/core#embodimentOf), a property representing an expression that is embodied by a manifestation."@en ,
                               "This property indicates that a particular manifestation embodies an expression of a work."@en ;
                  rdfs:isDefinedBy <http://purl.org/vocab/frbr/core> ;
                  rdfs:label "is embodiment of"@en .


###  http://purl.org/vocab/frbr/core#part
frbr:part rdf:type owl:ObjectProperty ;
          owl:inverseOf frbr:partOf ;
          rdfs:comment "Meaning = has part.  As defined by FRBR (http://www.ifla.org/VII/s13/frbr/frbr1.htm; http://purl.org/vocab/frbr/core#part),  a property indicating that one entity includes another entity."@en ;
          rdfs:isDefinedBy frbr: ;
          rdfs:label "has part"@en .


###  http://purl.org/vocab/frbr/core#partOf
frbr:partOf rdf:type owl:ObjectProperty ;
            rdfs:comment "Meaning = is part of.  As defined by FRBR (http://www.ifla.org/VII/s13/frbr/frbr1.htm; http://purl.org/vocab/frbr/core#partOf), a property indicating that one entity is a part of another entity."@en ;
            rdfs:isDefinedBy frbr: ;
            rdfs:label "is part of"@en .


###  http://purl.org/vocab/frbr/core#realization
frbr:realization rdf:type owl:ObjectProperty ;
                 owl:inverseOf frbr:realizationOf ;
                 rdfs:comment "As defined by FRBR (http://www.ifla.org/VII/s13/frbr/frbr1.htm; http://purl.org/vocab/frbr/core#realization), a property representing an expression that is an intellectual or artistic realization of a work."@en ;
                 rdfs:isDefinedBy frbr: ;
                 rdfs:label "has realization"@en .


###  http://purl.org/vocab/frbr/core#realizationOf
frbr:realizationOf rdf:type owl:ObjectProperty ,
                            owl:FunctionalProperty ;
                   rdfs:comment "As defined by FRBR (http://www.ifla.org/VII/s13/frbr/frbr1.htm; http://purl.org/vocab/frbr/core#realizationOf), a property representing the work that has been realized by an expression."@en ;
                   rdfs:isDefinedBy <http://purl.org/vocab/frbr/core> ;
                   rdfs:label "is realization of"@en .


###  http://www.essepuntato.it/2008/12/pattern#contains
<http://www.essepuntato.it/2008/12/pattern#contains> rdf:type owl:ObjectProperty ;
                                                     owl:inverseOf <http://www.essepuntato.it/2008/12/pattern#isContainedBy> ;
                                                     rdfs:comment "A structured element contains another generic element."@en ;
                                                     rdfs:isDefinedBy <http://www.essepuntato.it/2008/12/pattern#> ;
                                                     rdfs:label "contains"@en .


###  http://www.essepuntato.it/2008/12/pattern#isContainedBy
<http://www.essepuntato.it/2008/12/pattern#isContainedBy> rdf:type owl:ObjectProperty ;
                                                          rdfs:comment "An element that is contained by another structured element."@en ;
                                                          rdfs:label "is contained by"@en .


###  http://www.essepuntato.it/2012/04/tvc/atTime
<http://www.essepuntato.it/2012/04/tvc/atTime> rdf:type owl:ObjectProperty ;
                                               rdfs:comment "It specifies the particular temporal instant or time period in which the situation takes place."@en ;
                                               rdfs:isDefinedBy <http://www.essepuntato.it/2012/04/tvc/> ;
                                               rdfs:label "at time" .


###  https://w3id.org/arco/ontology/core/hasLocation
core:hasLocation rdf:type owl:ObjectProperty ;
                 owl:inverseOf core:isLocationOf ;
                 rdfs:domain owl:Thing ;
                 rdfs:comment "The object property that associates an entity to a location."@en ;
                 rdfs:isDefinedBy <https://w3id.org/arco/ontology/core> ;
                 rdfs:label "has location"@en .


###  https://w3id.org/arco/ontology/core/isLocationOf
core:isLocationOf rdf:type owl:ObjectProperty ;
                  rdfs:range owl:Thing ;
                  rdfs:comment "La object property che collega un luogo a un'entità che si trova in quel luogo."@it ,
                               "The object property that associates a location to an entity located there."@en ;
                  rdfs:isDefinedBy <https://w3id.org/arco/ontology/core> ;
                  rdfs:label "is location of"@en ,
                             "è luogo di"@it ;
                  owl:versionInfo "stabile"@it ,
                                  "stable"@en .


###  https://w3id.org/arco/ontology/location/hasLocationType
arco:hasLocationType rdf:type owl:ObjectProperty ;
                     owl:inverseOf arco:isLocationTypeOf ;
                     rdfs:domain owl:Thing ;
                     rdfs:range arco:LocationType ;
                     rdfs:comment "This property links an entity (e.g. a situation in which a place plays a certain role in relation to a cultural property in a time frame, or a georeferencing, or a cadastral identity) to the role of the localization referring to it (i.e current physical location, previous location, finding location, etc.)."@en ;
                     rdfs:isDefinedBy <https://w3id.org/arco/ontology/location> ;
                     rdfs:label "has referred location type"@en .


###  https://w3id.org/arco/ontology/location/isLocationTypeOf
arco:isLocationTypeOf rdf:type owl:ObjectProperty ;
                      rdfs:domain arco:LocationType ;
                      rdfs:range owl:Thing ;
                      rdfs:comment "This property links the role of a localization (i.e current physical location, previous location, finding location, etc.) to an entity referring to it (e.g. a situation in which a place plays a certain role in relation to a cultural property in a time frame, or a georeferencing, or a cadastral identity)."@en ;
                      rdfs:isDefinedBy <https://w3id.org/arco/ontology/location> ;
                      rdfs:label "is referred location type of"@en .


###  https://w3id.org/irnerio-mosaico/ontology/mmdio/hasBiography
:hasBiography rdf:type owl:ObjectProperty ;
              rdfs:comment "This relationship signifies that the document section provides or includes biographical information about an individual." ;
              rdfs:isDefinedBy <https://w3id.org/irnerio-mosaico/ontology/mmdio/> ;
              rdfs:label "has biography" .


###  https://w3id.org/irnerio-mosaico/ontology/mmdio/hasDecoration
:hasDecoration rdf:type owl:ObjectProperty ;
               rdfs:comment "An object property that connects a codex to its decorative elements, encompassing illustrations, borders, and other artistic features." ;
               rdfs:isDefinedBy <https://w3id.org/irnerio-mosaico/ontology/mmdio/> ;
               rdfs:label "has decoration" .


###  https://w3id.org/irnerio-mosaico/ontology/mmdio/hasDescription
:hasDescription rdf:type owl:ObjectProperty ;
                rdfs:comment "A textual representation that outlines the essential attributes, characteristics, and context of an entity or object." ;
                rdfs:isDefinedBy <https://w3id.org/irnerio-mosaico/ontology/mmdio/> ;
                rdfs:label "has description" .


###  https://w3id.org/irnerio-mosaico/ontology/mmdio/hasGlossPlacement
:hasGlossPlacement rdf:type owl:ObjectProperty ;
                   rdfs:comment "It indicates the placement of a gloss within a document." ;
                   rdfs:isDefinedBy <https://w3id.org/irnerio-mosaico/ontology/mmdio/> ;
                   rdfs:label "has gloss placement" .


###  https://w3id.org/irnerio-mosaico/ontology/mmdio/hasGlossType
:hasGlossType rdf:type owl:ObjectProperty ;
              rdfs:comment "It indicates the type or category of a gloss." ;
              rdfs:isDefinedBy <https://w3id.org/irnerio-mosaico/ontology/mmdio/> ;
              rdfs:label "has gloss type" .


###  https://w3id.org/irnerio-mosaico/ontology/mmdio/hasSection
:hasSection rdf:type owl:ObjectProperty ;
            rdfs:comment "A property indicating that an entity (e.g., a book or document) contains or is divided into smaller parts, known as sections. It establishes a hierarchical relationship between the whole and its components." ;
            rdfs:isDefinedBy <https://w3id.org/irnerio-mosaico/ontology/mmdio/> ;
            rdfs:label "has section" .


###  https://w3id.org/irnerio-mosaico/ontology/mmdio/isAbout
:isAbout rdf:type owl:ObjectProperty ;
         rdfs:comment "A property that identifies the primary subject of a piece of biographical information." ;
         rdfs:isDefinedBy <https://w3id.org/irnerio-mosaico/ontology/mmdio/> ;
         rdfs:label "is about" .


###  https://w3id.org/irnerio-mosaico/ontology/mmdio/refersToMenifestation
:refersToMenifestation rdf:type owl:ObjectProperty ;
                       rdfs:comment "A relationship that links an expression-level entity (e.g., document section) to a manifestation-level entity (e.g., folio). It captures the association from conceptual content to its physical or digital instantiation, enabling detailed metadata documentation for enhanced resource discoverability and navigability." ;
                       rdfs:isDefinedBy <https://w3id.org/irnerio-mosaico/ontology/mmdio/> ;
                       rdfs:label "refers to menifestation" .


###  https://w3id.org/irnerio/ontology/memo/hasSizeMeasurementUnit
memo:hasSizeMeasurementUnit rdf:type owl:ObjectProperty ;
                            rdfs:domain memo:SizeMeasurement ;
                            rdfs:range memo:SizeMeasurementUnit ;
                            rdfs:comment "This property indicates that an size is being measured with a certain size measurement unit."@en ;
                            rdfs:isDefinedBy <https://w3id.org/irnerio/ontology/memo> ;
                            rdfs:label "has size measurement unit"@en .


###  https://w3id.org/irnerio/ontology/memo/hasTextualMetadata
memo:hasTextualMetadata rdf:type owl:ObjectProperty ;
                        owl:inverseOf memo:isTextualMetadataOf ;
                        rdfs:comment "This property relates some resource to some textual metadata in time."@en ;
                        rdfs:isDefinedBy <https://w3id.org/irnerio/ontology/memo> ;
                        rdfs:label "has textual metadata"@en .


###  https://w3id.org/irnerio/ontology/memo/isTextualMetadataOf
memo:isTextualMetadataOf rdf:type owl:ObjectProperty ;
                         rdfs:comment "This property relates some textual metadata to some resource that has been provided with it." ;
                         rdfs:isDefinedBy <https://w3id.org/irnerio/ontology/memo> ;
                         rdfs:label "is textual metadata of" .


###  https://w3id.org/irnerio/ontology/memo/isTextualRoleIn
memo:isTextualRoleIn rdf:type owl:ObjectProperty ;
                     owl:inverseOf memo:withTextualRole ;
                     rdfs:comment "This property relates a textual role to the textual metadata with that role."@en ;
                     rdfs:isDefinedBy <https://w3id.org/irnerio/ontology/memo> ;
                     rdfs:label "is textual role in"@en .


###  https://w3id.org/irnerio/ontology/memo/withTextualRole
memo:withTextualRole rdf:type owl:ObjectProperty ;
                     rdfs:range memo:TextualRole ;
                     rdfs:comment "This property relates some textual metadata in time to its textual role."@en ;
                     rdfs:isDefinedBy <https://w3id.org/irnerio/ontology/memo> ;
                     rdfs:label "with textual role"@en .


#################################################################
#    Data properties
#################################################################

###  http://purl.org/dc/terms/identifier
dcterms:identifier rdf:type owl:DatatypeProperty ;
                   rdfs:comment "This property indicates a unique and unambiguous reference to the resource within a given context."@en ;
                   rdfs:isDefinedBy <http://purl.org/dc/terms> ;
                   rdfs:label "has identifier"@en .


###  http://purl.org/dc/terms/title
dcterms:title rdf:type owl:DatatypeProperty ;
              rdfs:comment "A name given to a resource.  Typically, the title will be the name by which the resource is formally known."@en ;
              rdfs:isDefinedBy <http://purl.org/dc/terms> ;
              rdfs:label "has title"@en .


###  http://purl.org/spar/c4o/hasContent
c4o:hasContent rdf:type owl:DatatypeProperty ;
               rdfs:subPropertyOf owl:topDataProperty ;
               rdfs:range rdfs:Literal ;
               rdfs:comment "It is used to specify the textual content of a particular FRBR expression."@en ;
               rdfs:isDefinedBy <http://purl.org/spar/c4o> ;
               rdfs:label "has content"@en .


###  http://www.ontologydesignpatterns.org/cp/owl/timeinterval.owl#hasIntervalEndDate
ti:hasIntervalEndDate rdf:type owl:DatatypeProperty ;
                      rdfs:domain ti:TimeInterval ;
                      rdfs:comment "The end date of a time interval." ;
                      rdfs:isDefinedBy <http://www.ontologydesignpatterns.org/cp/owl/timeinterval.owl> ;
                      rdfs:label "interval has end date"@en .


###  http://www.ontologydesignpatterns.org/cp/owl/timeinterval.owl#hasIntervalStartDate
ti:hasIntervalStartDate rdf:type owl:DatatypeProperty ;
                        rdfs:domain ti:TimeInterval ;
                        rdfs:comment "The start date of a time interval." ;
                        rdfs:isDefinedBy <http://www.ontologydesignpatterns.org/cp/owl/timeinterval.owl> ;
                        rdfs:label "interval has start date"@en .


###  http://xmlns.com/foaf/0.1/name
foaf:name rdf:type owl:DatatypeProperty ;
          rdfs:domain owl:Thing ;
          rdfs:range rdfs:Literal ;
          rdfs:comment "A name for some thing." ;
          rdfs:isDefinedBy foaf: ;
          rdfs:label "name" .


###  http://xmlns.com/foaf/0.1/nick
foaf:nick rdf:type owl:DatatypeProperty ;
          rdfs:comment "A short informal nickname characterising an agent (includes login identifiers, IRC and other chat nicknames)." ;
          rdfs:isDefinedBy foaf: ;
          rdfs:label "nickname" .


###  https://w3id.org/arco/ontology/core/description
core:description rdf:type owl:DatatypeProperty ;
                 rdfs:domain owl:Thing ;
                 rdfs:range rdfs:Literal ;
                 rdfs:comment "This property relates a description associated to an entity, in order to add details and some more information."@en ;
                 rdfs:isDefinedBy <https://w3id.org/arco/ontology/core> ;
                 rdfs:label "description"@en .


###  https://w3id.org/irnerio-mosaico/ontology/mmdio/hasFoliation
:hasFoliation rdf:type owl:DatatypeProperty ;
              rdfs:comment "A property that reference the arrangement and total count of folios in an item, detaliling their sequential order," ;
              rdfs:isDefinedBy <https://w3id.org/irnerio-mosaico/ontology/mmdio/> ;
              rdfs:label "has foliation" .


###  https://w3id.org/irnerio-mosaico/ontology/mmdio/hasInitial
:hasInitial rdf:type owl:DatatypeProperty ;
            rdfs:comment "An object property that relates a codex to its initial letters, specifically those that are enlarged or elaborately decorated at the beginning of sections or paragraphs." ;
            rdfs:isDefinedBy <https://w3id.org/irnerio-mosaico/ontology/mmdio/> ;
            rdfs:label "has initial" .


###  https://w3id.org/irnerio-mosaico/ontology/mmdio/hasLanguage
:hasLanguage rdf:type owl:DatatypeProperty ;
             rdfs:comment "A property identifies and stores the language information of a manuscript or text, using standardized codes to facilitate cataloging, search, and organization." ;
             rdfs:isDefinedBy <http://www.mmdio.org/ontology/mmdio> ;
             rdfs:label "has language" .


###  https://w3id.org/irnerio-mosaico/ontology/mmdio/hasLocationName
:hasLocationName rdf:type owl:DatatypeProperty ;
                 rdfs:comment "It stores the name of a specific place linked to a resource like a document, event, or object." ;
                 rdfs:isDefinedBy <https://w3id.org/irnerio-mosaico/ontology/mmdio/> ;
                 rdfs:label "has location name" .


###  https://w3id.org/irnerio-mosaico/ontology/mmdio/hasRubrication
:hasRubrication rdf:type owl:DatatypeProperty ;
                rdfs:comment "An object property that links a codex to the presence and details of rubrication, referring to the use of red ink for emphasis or decoration, such as in headings, initial letters, or other special text." ;
                rdfs:isDefinedBy <https://w3id.org/irnerio-mosaico/ontology/mmdio/> ;
                rdfs:label "has rubrication" .


###  https://w3id.org/irnerio-mosaico/ontology/mmdio/hasStyleScript
:hasStyleScript rdf:type owl:DatatypeProperty ;
                rdfs:comment "An object property that associates a codex with its particular style of script, indicating the type of calligraphy or font used." ;
                rdfs:isDefinedBy <https://w3id.org/irnerio-mosaico/ontology/mmdio/> ;
                rdfs:label "has style script" .


###  https://w3id.org/irnerio-mosaico/ontology/mmdio/hasTextualContent
:hasTextualContent rdf:type owl:DatatypeProperty ;
                   rdfs:comment "A data property that holds the textual content of features such as incipit, explicit , final rubric, follows and notes." ;
                   rdfs:isDefinedBy <https://w3id.org/irnerio-mosaico/ontology/mmdio/> ;
                   rdfs:label "has textual content" .


###  https://w3id.org/irnerio-mosaico/ontology/mmdio/hasWritingHands
:hasWritingHands rdf:type owl:DatatypeProperty ;
                 rdfs:comment "An object property that links a codex to the specific scribes or styles of handwriting found within it." ;
                 rdfs:isDefinedBy <https://w3id.org/irnerio-mosaico/ontology/mmdio/> ;
                 rdfs:label "has writing hands" .


###  https://w3id.org/irnerio/ontology/memo/hasLength
memo:hasLength rdf:type owl:DatatypeProperty ;
               rdfs:range xsd:positiveInteger ;
               rdfs:comment "This property indicates the size of something in terms of length."@en ;
               rdfs:isDefinedBy <https://w3id.org/irnerio/ontology/memo> ;
               rdfs:label "has length"@en .


###  https://w3id.org/irnerio/ontology/memo/hasNumberOfColumns
memo:hasNumberOfColumns rdf:type owl:DatatypeProperty ;
                        rdfs:domain memo:Side ;
                        rdfs:range xsd:positiveInteger ;
                        rdfs:comment "This property specifies the number of columns that are present on the side of a folio."@en ;
                        rdfs:isDefinedBy <https://w3id.org/irnerio/ontology/memo> ;
                        rdfs:label "has number of columns"@en .


###  https://w3id.org/irnerio/ontology/memo/hasWidth
memo:hasWidth rdf:type owl:DatatypeProperty ;
              rdfs:range xsd:positiveInteger ;
              rdfs:comment "This property indicates the size of something in terms of width."@en ;
              rdfs:isDefinedBy <https://w3id.org/irnerio/ontology/memo> ;
              rdfs:label "has width"@en .


#################################################################
#    Classes
#################################################################

###  http://purl.org/dc/terms/Location
dcterms:Location rdf:type owl:Class ;
                 rdfs:subClassOf [ rdf:type owl:Restriction ;
                                   owl:onProperty arco:hasLocationType ;
                                   owl:allValuesFrom arco:LocationType
                                 ] ,
                                 [ rdf:type owl:Restriction ;
                                   owl:onProperty :hasLocationName ;
                                   owl:qualifiedCardinality "1"^^xsd:nonNegativeInteger ;
                                   owl:onDataRange xsd:string
                                 ] ;
                 rdfs:comment "A spatial region or named place." ;
                 rdfs:isDefinedBy <http://purl.org/dc/terms> ;
                 rdfs:label "Location"@en-us .


###  http://purl.org/dc/terms/PhysicalMedium
dcterms:PhysicalMedium rdf:type owl:Class ;
                       rdfs:comment "A physical material or carrier."@en ;
                       rdfs:isDefinedBy <http://purl.org/dc/terms> ;
                       rdfs:label "Physical Medium"@en-us .


###  http://purl.org/dc/terms/SizeOrDuration
dcterms:SizeOrDuration rdf:type owl:Class ;
                       rdfs:comment "Examples include a number of pages, a specification of length, width, and breadth, or a period in hours, minutes, and seconds."@en-us ;
                       rdfs:isDefinedBy dcterms: ;
                       rdfs:label "Size or Duration"@en-us .


###  http://purl.org/spar/biro/BibliographicList
biro:BibliographicList rdf:type owl:Class ;
                       rdfs:subClassOf <http://purl.org/spar/fabio/Expression> ,
                                       [ rdf:type owl:Restriction ;
                                         owl:onProperty biro:references ;
                                         owl:minQualifiedCardinality "1"^^xsd:nonNegativeInteger ;
                                         owl:onClass biro:BibliographicReference
                                       ] ,
                                       [ rdf:type owl:Restriction ;
                                         owl:onProperty cito:cites ;
                                         owl:minQualifiedCardinality "1"^^xsd:nonNegativeInteger ;
                                         owl:onClass :ManuscriptCollection
                                       ] ;
                       rdfs:comment "An ordered list of bibliographic items, each of which contains a bibliographic reference."@en ;
                       rdfs:isDefinedBy <http://purl.org/spar/biro> ;
                       rdfs:label "bibliographic list"@en .


###  http://purl.org/spar/biro/BibliographicReference
biro:BibliographicReference rdf:type owl:Class ;
                            rdfs:subClassOf <http://purl.org/spar/fabio/Expression> ,
                                            [ rdf:type owl:Restriction ;
                                              owl:onProperty cito:cites ;
                                              owl:someValuesFrom <http://purl.org/spar/fabio/Book>
                                            ] ,
                                            [ rdf:type owl:Restriction ;
                                              owl:onProperty c4o:hasContent ;
                                              owl:cardinality "1"^^xsd:nonNegativeInteger
                                            ] ;
                            rdfs:comment "An expression of a bibliographic record in a specific format, that references a particular textual or data publication (or a work in preparation for publication). Each bibliographic reference is a list of items containing entities that describe aspects of the referenced work - for example authors, title, journal, publication year - selected from the bibliographic record."@en ;
                            rdfs:isDefinedBy <http://purl.org/spar/biro> ;
                            rdfs:label "bibliographic reference"@en .


###  http://purl.org/spar/deo/Biography
deo:Biography rdf:type owl:Class ;
              rdfs:subClassOf [ rdf:type owl:Restriction ;
                                owl:onProperty :isAbout ;
                                owl:allValuesFrom foaf:Person
                              ] ,
                              [ rdf:type owl:Restriction ;
                                owl:onProperty core:description ;
                                owl:maxQualifiedCardinality "1"^^xsd:nonNegativeInteger ;
                                owl:onDataRange xsd:string
                              ] ;
              rdfs:comment "Information describing a person and his or her life history and contributions."@en ;
              rdfs:isDefinedBy deo: ;
              rdfs:label "biography"@en .


###  http://purl.org/spar/deo/SupplementaryInformationDescription
deo:SupplementaryInformationDescription rdf:type owl:Class ;
                                        rdfs:subClassOf [ rdf:type owl:Restriction ;
                                                          owl:onProperty core:description ;
                                                          owl:qualifiedCardinality "1"^^xsd:nonNegativeInteger ;
                                                          owl:onDataRange xsd:string
                                                        ] ;
                                        rdfs:comment "Information describing supplementary information relating to the document, including references or links to the relevant supplementary information."@en ;
                                        rdfs:isDefinedBy <http://purl.org/spar/deo> ;
                                        rdfs:label "supplementary information description"@en .


###  http://purl.org/spar/doco/Section
<http://purl.org/spar/doco/Section> rdf:type owl:Class ;
                                    rdfs:subClassOf <http://purl.org/spar/fabio/Expression> ,
                                                    [ rdf:type owl:Restriction ;
                                                      owl:onProperty cito:cites ;
                                                      owl:someValuesFrom biro:BibliographicList
                                                    ] ,
                                                    [ rdf:type owl:Restriction ;
                                                      owl:onProperty :hasBiography ;
                                                      owl:someValuesFrom deo:Biography
                                                    ] ,
                                                    [ rdf:type owl:Restriction ;
                                                      owl:onProperty dcterms:title ;
                                                      owl:cardinality "1"^^xsd:nonNegativeInteger
                                                    ] ,
                                                    [ rdf:type owl:Restriction ;
                                                      owl:onProperty core:description ;
                                                      owl:qualifiedCardinality "1"^^xsd:nonNegativeInteger ;
                                                      owl:onDataRange xsd:string
                                                    ] ;
                                    rdfs:comment "A logical division of the text, usually numbered and/or titled, which may contain subsections."@en ;
                                    rdfs:isDefinedBy <http://purl.org/spar/doco> ;
                                    rdfs:label "section"@en .


###  http://purl.org/spar/fabio/Book
<http://purl.org/spar/fabio/Book> rdf:type owl:Class ;
                                  rdfs:subClassOf <http://purl.org/spar/fabio/Expression> ,
                                                  [ rdf:type owl:Restriction ;
                                                    owl:onProperty cito:cites ;
                                                    owl:someValuesFrom :ManuscriptCollection
                                                  ] ,
                                                  [ rdf:type owl:Restriction ;
                                                    owl:onProperty cito:cites ;
                                                    owl:someValuesFrom memo:Manuscript
                                                  ] ,
                                                  [ rdf:type owl:Restriction ;
                                                    owl:onProperty :hasSection ;
                                                    owl:someValuesFrom <http://purl.org/spar/doco/Section>
                                                  ] ,
                                                  [ rdf:type owl:Restriction ;
                                                    owl:onProperty dcterms:creator ;
                                                    owl:qualifiedCardinality "1"^^xsd:nonNegativeInteger ;
                                                    owl:onClass foaf:Person
                                                  ] ,
                                                  [ rdf:type owl:Restriction ;
                                                    owl:onProperty frbr:partOf ;
                                                    owl:qualifiedCardinality "1"^^xsd:nonNegativeInteger ;
                                                    owl:onClass :DigitalResourceCollection
                                                  ] ,
                                                  [ rdf:type owl:Restriction ;
                                                    owl:onProperty <http://www.essepuntato.it/2012/04/tvc/atTime> ;
                                                    owl:maxQualifiedCardinality "1"^^xsd:nonNegativeInteger ;
                                                    owl:onClass ti:TimeInterval
                                                  ] ,
                                                  [ rdf:type owl:Restriction ;
                                                    owl:onProperty dcterms:title ;
                                                    owl:cardinality "1"^^xsd:nonNegativeInteger
                                                  ] ;
                                  rdfs:comment "A non-serial document that is complete in one volume or a designated finite number of volumes.  A book published by a publisher is usually  identified by an International Standard Book Number (ISBN), and may be manifested as a physical printed publication on paper bound in a hard or soft cover, or in electronic format as an 'e-book'."@en ;
                                  rdfs:isDefinedBy <http://purl.org/spar/fabio/> ;
                                  rdfs:label "book"@en .


###  http://purl.org/spar/fabio/Comment
<http://purl.org/spar/fabio/Comment> rdf:type owl:Class ;
                                     rdfs:subClassOf <http://purl.org/spar/fabio/Expression> ,
                                                     [ rdf:type owl:Restriction ;
                                                       owl:onProperty cito:cites ;
                                                       owl:allValuesFrom <http://purl.org/spar/fabio/Book>
                                                     ] ,
                                                     [ rdf:type owl:Restriction ;
                                                       owl:onProperty cito:cites ;
                                                       owl:allValuesFrom memo:Text
                                                     ] ,
                                                     [ rdf:type owl:Restriction ;
                                                       owl:onProperty cito:cites ;
                                                       owl:allValuesFrom [ rdf:type owl:Class ;
                                                                           owl:unionOf ( <http://purl.org/spar/fabio/Book>
                                                                                         memo:Text
                                                                                       )
                                                                         ]
                                                     ] ;
                                     rdfs:comment "A verbal or written remark concerning some entity.  In written form, a comment is often appended to that entity and termed an annotation.  Within computer programs or ontologies, comments are added to enhance human understanding, and are usually prefaced by a special syntactic symbol that ensures they are ignored during execution of the program."@en ;
                                     rdfs:isDefinedBy <http://purl.org/spar/fabio/> ;
                                     rdfs:label "comment"@en .


###  http://purl.org/spar/fabio/CriticalEdition
<http://purl.org/spar/fabio/CriticalEdition> rdf:type owl:Class ;
                                             rdfs:subClassOf <http://purl.org/spar/fabio/Work> ,
                                                             [ rdf:type owl:Restriction ;
                                                               owl:onProperty frbr:realization ;
                                                               owl:allValuesFrom memo:CriticalEditionVolume
                                                             ] ,
                                                             [ rdf:type owl:Restriction ;
                                                               owl:onProperty dcterms:title ;
                                                               owl:maxCardinality "1"^^xsd:nonNegativeInteger
                                                             ] ;
                                             rdfs:comment "A new edition of a historical publication, edited by a scholar other than the original author, containing within the body text the supposedly best version of the original work, with footnotes detailing and commenting on textual variations between different versions, typically with an introduction to the original work written by the scholar, and with a bibliography listing related publications."@en ;
                                             rdfs:isDefinedBy <http://purl.org/spar/fabio> ;
                                             rdfs:label "critical edition"@en .


###  http://purl.org/spar/fabio/Expression
<http://purl.org/spar/fabio/Expression> rdf:type owl:Class ;
                                        rdfs:subClassOf [ rdf:type owl:Restriction ;
                                                          owl:onProperty frbr:embodiment ;
                                                          owl:allValuesFrom <http://purl.org/spar/fabio/Manifestation>
                                                        ] ,
                                                        [ rdf:type owl:Restriction ;
                                                          owl:onProperty frbr:realizationOf ;
                                                          owl:allValuesFrom <http://purl.org/spar/fabio/Work>
                                                        ] ;
                                        rdfs:comment "A subclass of FRBR expression, restricted to expressions of fabio:Works.  For your latest research paper, the preprint submitted to the publisher, and the final published version to which the publisher assigned a unique digital object identifier, are both expressions of the same work.  "@en ;
                                        rdfs:isDefinedBy <http://purl.org/spar/fabio> ;
                                        rdfs:label "expression"@en .


###  http://purl.org/spar/fabio/Manifestation
<http://purl.org/spar/fabio/Manifestation> rdf:type owl:Class ;
                                           rdfs:subClassOf [ rdf:type owl:Restriction ;
                                                             owl:onProperty frbr:embodimentOf ;
                                                             owl:allValuesFrom <http://purl.org/spar/fabio/Expression>
                                                           ] ;
                                           rdfs:comment """A subclass of FRBR manifestation, restricted to manifestations of fabio:Expressions. fabio:Manifestation specifically applies to electronic (digital) as well as to physical manifestations of expressions.  

Examples of different manifestations of a single 'version of record' expression of a scholarly work include an article in a print journal or the on-line version of that article as a web page."""@en ;
                                           rdfs:isDefinedBy <http://purl.org/spar/fabio> ;
                                           rdfs:label "manifestation"@en .


###  http://purl.org/spar/fabio/Work
<http://purl.org/spar/fabio/Work> rdf:type owl:Class ;
                                  rdfs:subClassOf [ rdf:type owl:Restriction ;
                                                    owl:onProperty frbr:realization ;
                                                    owl:allValuesFrom <http://purl.org/spar/fabio/Expression>
                                                  ] ;
                                  rdfs:comment "A subclass of FRBR work, restricted to works that are published or potentially publishable, and that contain or are referred to by bibliographic references, or entities used to define bibliographic references. FaBiO works, and their expressions and manifestations, are primarily textual publications such as books, magazines, newspapers and journals, and items of their content.  However, they also include datasets, computer algorithms, experimental protocols, formal specifications and vocabularies, legal records, governmental papers, technical and commercial reports and similar publications, and also bibliographies, reference lists, library catalogues and similar collections. For this reason, fabio:Work is not an equivalent class to frbr:ScholarlyWork.  An example of a fabio:Work is your latest research paper."@en ;
                                  rdfs:label "work"@en .


###  http://www.ontologydesignpatterns.org/cp/owl/timeinterval.owl#TimeInterval
ti:TimeInterval rdf:type owl:Class ;
                rdfs:subClassOf [ rdf:type owl:Restriction ;
                                  owl:onProperty ti:hasIntervalEndDate ;
                                  owl:maxCardinality "1"^^xsd:nonNegativeInteger
                                ] ,
                                [ rdf:type owl:Restriction ;
                                  owl:onProperty ti:hasIntervalStartDate ;
                                  owl:maxCardinality "1"^^xsd:nonNegativeInteger
                                ] ;
                rdfs:comment """Any Region in a dimensional space that aims at representing time.
It should be used when you want to talk about time as an object having some characteristics.""" ;
                rdfs:isDefinedBy <http://www.ontologydesignpatterns.org/cp/owl/timeinterval.owl> ;
                rdfs:label "Time interval"@en .


###  http://xmlns.com/foaf/0.1/Agent
foaf:Agent rdf:type owl:Class ;
           rdfs:comment "An agent (eg. person, group, software or physical artifact)." ;
           rdfs:isDefinedBy foaf: ;
           rdfs:label "Agent" .


###  http://xmlns.com/foaf/0.1/Organization
foaf:Organization rdf:type owl:Class ;
                  rdfs:subClassOf [ rdf:type owl:Restriction ;
                                    owl:onProperty foaf:name ;
                                    owl:cardinality "1"^^xsd:nonNegativeInteger
                                  ] ;
                  owl:disjointWith foaf:Person ;
                  rdfs:comment "An organization." ;
                  rdfs:isDefinedBy foaf: ;
                  rdfs:label "Organization" .


###  http://xmlns.com/foaf/0.1/Person
foaf:Person rdf:type owl:Class ;
            rdfs:subClassOf foaf:Agent ,
                            [ rdf:type owl:Restriction ;
                              owl:onProperty foaf:name ;
                              owl:cardinality "1"^^xsd:nonNegativeInteger
                            ] ,
                            [ rdf:type owl:Restriction ;
                              owl:onProperty foaf:nick ;
                              owl:cardinality "1"^^xsd:nonNegativeInteger
                            ] ;
            rdfs:comment "A person." ;
            rdfs:isDefinedBy foaf: ;
            rdfs:label "Person" .


###  https://w3id.org/arco/ontology/location/LocationType
arco:LocationType rdf:type owl:Class ;
                  rdfs:subClassOf [ rdf:type owl:Restriction ;
                                    owl:onProperty arco:isLocationTypeOf ;
                                    owl:someValuesFrom owl:Thing
                                  ] ;
                  rdfs:comment "Questa classe rappresenta il tipo di localizzazione di un bene culturale."@it ,
                               "This class represents the type of location of a cultural property."@en ;
                  rdfs:isDefinedBy <https://w3id.org/arco/ontology/location> ;
                  rdfs:label "Location Type"@en ,
                             "Tipo di localizzazione"@it ;
                  owl:versionInfo "stabile"@it ,
                                  "stable"@en .


###  https://w3id.org/irnerio-mosaico/ontology/mmdio/Decoration
:Decoration rdf:type owl:Class ;
            rdfs:subClassOf <http://purl.org/spar/fabio/Manifestation> ,
                            [ rdf:type owl:Restriction ;
                              owl:onProperty :hasInitial ;
                              owl:minQualifiedCardinality "1"^^xsd:nonNegativeInteger ;
                              owl:onDataRange xsd:string
                            ] ,
                            [ rdf:type owl:Restriction ;
                              owl:onProperty :hasRubrication ;
                              owl:minQualifiedCardinality "1"^^xsd:nonNegativeInteger ;
                              owl:onDataRange xsd:string
                            ] ;
            rdfs:comment "A class representing the various types of artistic embellishments or ornamental designs found in a codex, such as illustrations, miniatures, and ornate borders." ;
            rdfs:isDefinedBy <https://w3id.org/irnerio-mosaico/ontology/mmdio/> ;
            rdfs:label "decoration" .


###  https://w3id.org/irnerio-mosaico/ontology/mmdio/DigitalResourceCollection
:DigitalResourceCollection rdf:type owl:Class ;
                           rdfs:subClassOf <http://purl.org/spar/fabio/Expression> ,
                                           [ rdf:type owl:Restriction ;
                                             owl:onProperty dcterms:creator ;
                                             owl:maxQualifiedCardinality "1"^^xsd:nonNegativeInteger ;
                                             owl:onClass foaf:Organization
                                           ] ,
                                           [ rdf:type owl:Restriction ;
                                             owl:onProperty <http://www.essepuntato.it/2012/04/tvc/atTime> ;
                                             owl:maxQualifiedCardinality "1"^^xsd:nonNegativeInteger ;
                                             owl:onClass ti:TimeInterval
                                           ] ,
                                           [ rdf:type owl:Restriction ;
                                             owl:onProperty dcterms:title ;
                                             owl:cardinality "1"^^xsd:nonNegativeInteger
                                           ] ;
                           rdfs:comment "It represents the medieval manuscript information integrated from heterogeneous sources." ;
                           rdfs:isDefinedBy <https://w3id.org/irnerio-mosaico/ontology/mmdio/> ;
                           rdfs:label "digital resource collection" .


###  https://w3id.org/irnerio-mosaico/ontology/mmdio/GlossPlacement
:GlossPlacement rdf:type owl:Class ;
                rdfs:subClassOf <http://purl.org/spar/fabio/Expression> ;
                rdfs:comment "It represents the placement attribute of glosses in a document." ;
                rdfs:isDefinedBy <http://www.mmdio.org/ontology/mmdio> ;
                rdfs:label "gloss placement" .


###  https://w3id.org/irnerio-mosaico/ontology/mmdio/GlossType
:GlossType rdf:type owl:Class ;
           rdfs:subClassOf <http://purl.org/spar/fabio/Expression> ;
           rdfs:comment "It represents the categorization of glosses based on their characteristics." ;
           rdfs:isDefinedBy <http://www.mmdio.org/ontology/mmdio> ;
           rdfs:label "gloss type" .


###  https://w3id.org/irnerio-mosaico/ontology/mmdio/ManuscriptCollection
:ManuscriptCollection rdf:type owl:Class ;
                      rdfs:subClassOf <http://purl.org/spar/fabio/Expression> ,
                                      [ rdf:type owl:Restriction ;
                                        owl:onProperty frbr:embodiment ;
                                        owl:allValuesFrom memo:Codex
                                      ] ,
                                      [ rdf:type owl:Restriction ;
                                        owl:onProperty frbr:partOf ;
                                        owl:allValuesFrom :DigitalResourceCollection
                                      ] ,
                                      [ rdf:type owl:Restriction ;
                                        owl:onProperty frbr:part ;
                                        owl:minQualifiedCardinality "1"^^xsd:nonNegativeInteger ;
                                        owl:onClass memo:Manuscript
                                      ] ,
                                      [ rdf:type owl:Restriction ;
                                        owl:onProperty :hasDescription ;
                                        owl:minQualifiedCardinality "1"^^xsd:nonNegativeInteger ;
                                        owl:onClass deo:SupplementaryInformationDescription
                                      ] ,
                                      [ rdf:type owl:Restriction ;
                                        owl:onProperty <http://www.essepuntato.it/2012/04/tvc/atTime> ;
                                        owl:maxQualifiedCardinality "1"^^xsd:nonNegativeInteger ;
                                        owl:onClass ti:TimeInterval
                                      ] ,
                                      [ rdf:type owl:Restriction ;
                                        owl:onProperty core:hasLocation ;
                                        owl:maxQualifiedCardinality "2"^^xsd:nonNegativeInteger ;
                                        owl:onClass dcterms:Location
                                      ] ,
                                      [ rdf:type owl:Restriction ;
                                        owl:onProperty dcterms:title ;
                                        owl:cardinality "1"^^xsd:nonNegativeInteger
                                      ] ;
                      rdfs:comment "A Manuscript Collection is a compilation of handwritten documents, especially focusing on medieval manuscripts. These collections encompass a range of historically or culturally significant items, such as ancient scrolls, medieval codices, and other hand-crafted documents, reflecting the rich heritage and knowledge of the periods they originate from" ;
                      rdfs:isDefinedBy <https://w3id.org/irnerio-mosaico/ontology/mmdio/> ;
                      rdfs:label "manuscript collection" .


###  https://w3id.org/irnerio-mosaico/ontology/mmdio/TextualMetadata
:TextualMetadata rdf:type owl:Class ;
                 rdfs:subClassOf [ rdf:type owl:Restriction ;
                                   owl:onProperty memo:withTextualRole ;
                                   owl:allValuesFrom memo:TextualRole
                                 ] ,
                                 [ rdf:type owl:Restriction ;
                                   owl:onProperty :hasTextualContent ;
                                   owl:qualifiedCardinality "1"^^xsd:nonNegativeInteger ;
                                   owl:onDataRange xsd:string
                                 ] ;
                 rdfs:comment "It refers to data that provides contextual or supplementary information about a text." ;
                 rdfs:isDefinedBy <https://w3id.org/irnerio-mosaico/ontology/mmdio/> ;
                 rdfs:label "textual metadata" .


###  https://w3id.org/irnerio/ontology/memo/Binding
memo:Binding rdf:type owl:Class ;
             rdfs:subClassOf <http://purl.org/spar/fabio/Manifestation> ,
                             [ rdf:type owl:Restriction ;
                               owl:onProperty dcterms:extent ;
                               owl:allValuesFrom memo:SizeMeasurement
                             ] ,
                             [ rdf:type owl:Restriction ;
                               owl:onProperty dcterms:medium ;
                               owl:allValuesFrom dcterms:PhysicalMedium
                             ] ;
             rdfs:comment "The structure that holds a codex together."@en ;
             rdfs:isDefinedBy <https://w3id.org/irnerio/ontology/memo> ;
             rdfs:label "binding"@en .


###  https://w3id.org/irnerio/ontology/memo/Codex
memo:Codex rdf:type owl:Class ;
           rdfs:subClassOf <http://purl.org/spar/fabio/Manifestation> ,
                           [ rdf:type owl:Restriction ;
                             owl:onProperty :hasDecoration ;
                             owl:someValuesFrom :Decoration
                           ] ,
                           [ rdf:type owl:Restriction ;
                             owl:onProperty frbr:part ;
                             owl:allValuesFrom memo:Binding
                           ] ,
                           [ rdf:type owl:Restriction ;
                             owl:onProperty frbr:part ;
                             owl:allValuesFrom memo:Folio
                           ] ,
                           [ rdf:type owl:Restriction ;
                             owl:onProperty frbr:part ;
                             owl:allValuesFrom [ rdf:type owl:Class ;
                                                 owl:unionOf ( memo:Binding
                                                               memo:Folio
                                                             )
                                               ]
                           ] ,
                           [ rdf:type owl:Restriction ;
                             owl:onProperty :hasStyleScript ;
                             owl:minQualifiedCardinality "1"^^xsd:nonNegativeInteger ;
                             owl:onDataRange xsd:string
                           ] ,
                           [ rdf:type owl:Restriction ;
                             owl:onProperty :hasWritingHands ;
                             owl:minQualifiedCardinality "1"^^xsd:nonNegativeInteger ;
                             owl:onDataRange xsd:string
                           ] ,
                           [ rdf:type owl:Restriction ;
                             owl:onProperty dcterms:identifier ;
                             owl:cardinality "1"^^xsd:nonNegativeInteger
                           ] ,
                           [ rdf:type owl:Restriction ;
                             owl:onProperty :hasFoliation ;
                             owl:cardinality "1"^^xsd:nonNegativeInteger
                           ] ;
           rdfs:comment "A book constructed of one or more folios and at most one binding."@en ;
           rdfs:isDefinedBy <https://w3id.org/irnerio/ontology/memo> ;
           rdfs:label "codex"@en .


###  https://w3id.org/irnerio/ontology/memo/CriticalEditionVolume
memo:CriticalEditionVolume rdf:type owl:Class ;
                           rdfs:subClassOf <http://purl.org/spar/fabio/Expression> ,
                                           [ rdf:type owl:Restriction ;
                                             owl:onProperty cito:cites ;
                                             owl:allValuesFrom memo:Manuscript
                                           ] ,
                                           [ rdf:type owl:Restriction ;
                                             owl:onProperty dcterms:identifier ;
                                             owl:cardinality "1"^^xsd:nonNegativeInteger
                                           ] ;
                           rdfs:comment "The specific realization of a critical edition."@en ;
                           rdfs:isDefinedBy <https://w3id.org/irnerio/ontology/memo> ;
                           rdfs:label "critical edition volume"@en .


###  https://w3id.org/irnerio/ontology/memo/Folio
memo:Folio rdf:type owl:Class ;
           rdfs:subClassOf <http://purl.org/spar/fabio/Manifestation> ,
                           [ rdf:type owl:Restriction ;
                             owl:onProperty dcterms:extent ;
                             owl:allValuesFrom memo:SizeMeasurement
                           ] ,
                           [ rdf:type owl:Restriction ;
                             owl:onProperty dcterms:medium ;
                             owl:allValuesFrom dcterms:PhysicalMedium
                           ] ,
                           [ rdf:type owl:Restriction ;
                             owl:onProperty frbr:part ;
                             owl:allValuesFrom memo:Recto
                           ] ,
                           [ rdf:type owl:Restriction ;
                             owl:onProperty frbr:part ;
                             owl:allValuesFrom memo:Side
                           ] ,
                           [ rdf:type owl:Restriction ;
                             owl:onProperty frbr:part ;
                             owl:allValuesFrom memo:Verso
                           ] ;
           rdfs:comment "The page of a codex. It is made up by two sides, called respectively recto and verso."@en ;
           rdfs:isDefinedBy <https://w3id.org/irnerio/ontology/memo> ;
           rdfs:label "folio"@en .


###  https://w3id.org/irnerio/ontology/memo/Gloss
memo:Gloss rdf:type owl:Class ;
           rdfs:subClassOf <http://purl.org/spar/fabio/Comment> ,
                           [ rdf:type owl:Restriction ;
                             owl:onProperty frbr:embodiment ;
                             owl:allValuesFrom memo:Folio
                           ] ,
                           [ rdf:type owl:Restriction ;
                             owl:onProperty :hasGlossPlacement ;
                             owl:qualifiedCardinality "1"^^xsd:nonNegativeInteger ;
                             owl:onClass :GlossPlacement
                           ] ,
                           [ rdf:type owl:Restriction ;
                             owl:onProperty :hasGlossType ;
                             owl:qualifiedCardinality "1"^^xsd:nonNegativeInteger ;
                             owl:onClass :GlossType
                           ] ,
                           [ rdf:type owl:Restriction ;
                             owl:onProperty :hasDescription ;
                             owl:maxQualifiedCardinality "1"^^xsd:nonNegativeInteger ;
                             owl:onClass deo:SupplementaryInformationDescription
                           ] ,
                           [ rdf:type owl:Restriction ;
                             owl:onProperty dcterms:identifier ;
                             owl:cardinality "1"^^xsd:nonNegativeInteger
                           ] ,
                           [ rdf:type owl:Restriction ;
                             owl:onProperty dcterms:title ;
                             owl:cardinality "1"^^xsd:nonNegativeInteger
                           ] ;
           rdfs:comment "An annotation that is part of a manuscript. It consists of a brief explanation or a continuous commentary accompanying a manuscript text (as in the margin or between the lines of the text)."@en ;
           rdfs:isDefinedBy <https://w3id.org/irnerio/ontology/memo> ;
           rdfs:label "gloss"@en .


###  https://w3id.org/irnerio/ontology/memo/Manuscript
memo:Manuscript rdf:type owl:Class ;
                rdfs:subClassOf <http://purl.org/spar/fabio/Book> ,
                                [ rdf:type owl:Restriction ;
                                  owl:onProperty frbr:part ;
                                  owl:allValuesFrom memo:Text
                                ] ,
                                [ rdf:type owl:Restriction ;
                                  owl:onProperty frbr:part ;
                                  owl:allValuesFrom [ rdf:type owl:Class ;
                                                      owl:unionOf ( memo:Gloss
                                                                    memo:Text
                                                                  )
                                                    ]
                                ] ,
                                [ rdf:type owl:Restriction ;
                                  owl:onProperty memo:hasTextualMetadata ;
                                  owl:allValuesFrom :TextualMetadata
                                ] ,
                                [ rdf:type owl:Restriction ;
                                  owl:onProperty core:hasLocation ;
                                  owl:maxQualifiedCardinality "2"^^xsd:nonNegativeInteger ;
                                  owl:onClass dcterms:Location
                                ] ,
                                [ rdf:type owl:Restriction ;
                                  owl:onProperty :hasLanguage ;
                                  owl:qualifiedCardinality "1"^^xsd:nonNegativeInteger ;
                                  owl:onDataRange xsd:string
                                ] ;
                rdfs:comment "A handwritten composition constructed of one text and zero or more glosses."@en ;
                rdfs:isDefinedBy <https://w3id.org/irnerio/ontology/memo> ;
                rdfs:label "manuscript"@en .


###  https://w3id.org/irnerio/ontology/memo/Recto
memo:Recto rdf:type owl:Class ;
           rdfs:subClassOf memo:Side ,
                           [ rdf:type owl:Restriction ;
                             owl:onProperty dcterms:identifier ;
                             owl:cardinality "1"^^xsd:nonNegativeInteger
                           ] ;
           rdfs:comment "The side of a folio that usually (but not necessarily) is to be read first."@en ;
           rdfs:isDefinedBy <https://w3id.org/irnerio/ontology/memo> ;
           rdfs:label "recto"@en .


###  https://w3id.org/irnerio/ontology/memo/Side
memo:Side rdf:type owl:Class ;
          rdfs:subClassOf <http://purl.org/spar/fabio/Manifestation> ,
                          [ rdf:type owl:Restriction ;
                            owl:onProperty memo:hasNumberOfColumns ;
                            owl:cardinality "1"^^xsd:nonNegativeInteger
                          ] ;
          rdfs:comment "A single side of a folio."@en ;
          rdfs:isDefinedBy <https://w3id.org/irnerio/ontology/memo> ;
          rdfs:label "side"@en .


###  https://w3id.org/irnerio/ontology/memo/SizeMeasurement
memo:SizeMeasurement rdf:type owl:Class ;
                     rdfs:subClassOf dcterms:SizeOrDuration ,
                                     [ rdf:type owl:Restriction ;
                                       owl:onProperty memo:hasSizeMeasurementUnit ;
                                       owl:allValuesFrom memo:SizeMeasurementUnit
                                     ] ,
                                     [ rdf:type owl:Restriction ;
                                       owl:onProperty memo:hasLength ;
                                       owl:cardinality "1"^^xsd:nonNegativeInteger
                                     ] ,
                                     [ rdf:type owl:Restriction ;
                                       owl:onProperty memo:hasWidth ;
                                       owl:cardinality "1"^^xsd:nonNegativeInteger
                                     ] ;
                     rdfs:comment "The amount of space or surface that something occupies or the distance over which it extends."@en ;
                     rdfs:isDefinedBy <https://w3id.org/irnerio/ontology/memo> ;
                     rdfs:label "size measurement"@en .


###  https://w3id.org/irnerio/ontology/memo/SizeMeasurementUnit
memo:SizeMeasurementUnit rdf:type owl:Class ;
                         rdfs:comment "The definite magnitude of a quantity, defined and adopted by convention or by law, that is used as a standard for measurement of size."@en ;
                         rdfs:isDefinedBy <https://w3id.org/irnerio/ontology/memo> ;
                         rdfs:label "size measurement unit"@en .


###  https://w3id.org/irnerio/ontology/memo/Text
memo:Text rdf:type owl:Class ;
          rdfs:subClassOf <http://purl.org/spar/fabio/Expression> ,
                          [ rdf:type owl:Restriction ;
                            owl:onProperty frbr:embodiment ;
                            owl:allValuesFrom memo:Folio
                          ] ,
                          [ rdf:type owl:Restriction ;
                            owl:onProperty frbr:partOf ;
                            owl:allValuesFrom memo:Manuscript
                          ] ;
          rdfs:comment "The primary text that is part of a manuscript."@en ;
          rdfs:isDefinedBy <https://w3id.org/irnerio/ontology/memo> ;
          rdfs:label "text"@en .


###  https://w3id.org/irnerio/ontology/memo/TextualRole
memo:TextualRole rdf:type owl:Class ;
                 rdfs:comment "A function assumed by some textual metadata in time. A textual metadata in time can assume the role of either incipit, explicit or final rubric."@en ;
                 rdfs:isDefinedBy <https://w3id.org/irnerio/ontology/memo> ;
                 rdfs:label "textual role"@en .


###  https://w3id.org/irnerio/ontology/memo/Verso
memo:Verso rdf:type owl:Class ;
           rdfs:subClassOf memo:Side ,
                           [ rdf:type owl:Restriction ;
                             owl:onProperty dcterms:identifier ;
                             owl:cardinality "1"^^xsd:nonNegativeInteger
                           ] ;
           rdfs:comment "The side of a folio that usually (but not necessarily) is to be read second."@en ;
           rdfs:isDefinedBy <https://w3id.org/irnerio/ontology/memo> ;
           rdfs:label "verso"@en .


#################################################################
#    Individuals
#################################################################

###  https://w3id.org/arco/ontology/location/CurrentPhysicalLocation
arco:CurrentPhysicalLocation rdf:type owl:NamedIndividual ,
                                      arco:LocationType ;
                             rdfs:comment "This individual represents a specific type of localization, that is the current physical location."@en ;
                             rdfs:isDefinedBy <https://w3id.org/arco/ontology/location> ;
                             rdfs:label "Current Physical Location"@en .


###  https://w3id.org/arco/ontology/location/PreviousLocation
arco:PreviousLocation rdf:type owl:NamedIndividual ,
                               arco:LocationType ;
                      rdfs:comment "This individual represents a specific type of location, that is the place of origin or previous location."@en ;
                      rdfs:isDefinedBy <https://w3id.org/arco/ontology/location> ;
                      rdfs:label "Place of Origin / Previous Location"@en .


###  https://w3id.org/irnerio-mosaico/ontology/mmdio/extravagant
:extravagant rdf:type owl:NamedIndividual ,
                      :GlossType ;
             rdfs:comment "An individual that exemplifies glosses which are unusual or beyond the standard scope." ;
             rdfs:isDefinedBy <https://w3id.org/irnerio-mosaico/ontology/mmdio/> ;
             rdfs:label "extravagant" .


###  https://w3id.org/irnerio-mosaico/ontology/mmdio/follows
:follows rdf:type owl:NamedIndividual ,
                  memo:TextualRole ;
         rdfs:comment "A relational property used to indicate that one section or element in a manuscript directly comes after another in the sequence." ;
         rdfs:isDefinedBy <https://w3id.org/irnerio-mosaico/ontology/mmdio/> ;
         rdfs:label "follows" .


###  https://w3id.org/irnerio-mosaico/ontology/mmdio/interlinear
:interlinear rdf:type owl:NamedIndividual ,
                      :GlossPlacement ;
             rdfs:comment "An individual that represents glosses placed between the lines of text on a page." ;
             rdfs:isDefinedBy <https://w3id.org/irnerio-mosaico/ontology/mmdio/> ;
             rdfs:label "interlinear" .


###  https://w3id.org/irnerio-mosaico/ontology/mmdio/marginal
:marginal rdf:type owl:NamedIndividual ,
                   :GlossPlacement ;
          rdfs:comment "An individual that represents glosses placed in the margins of a page." ;
          rdfs:isDefinedBy <https://w3id.org/irnerio-mosaico/ontology/mmdio/> ;
          rdfs:label "marginal" .


###  https://w3id.org/irnerio-mosaico/ontology/mmdio/notes
:notes rdf:type owl:NamedIndividual ,
                memo:TextualRole ;
       rdfs:comment "Supplementary information or annotations that provide additional insight, clarification, or commentary on the main text or its parts. These might include scholarly notes, historical context, or corrections." ;
       rdfs:isDefinedBy <https://w3id.org/irnerio-mosaico/ontology/mmdio/> ;
       rdfs:label "notes" .


###  https://w3id.org/irnerio-mosaico/ontology/mmdio/ordinary
:ordinary rdf:type owl:NamedIndividual ,
                   :GlossType ;
          rdfs:comment "An individual that exemplifies standard or typical glosses." ;
          rdfs:isDefinedBy <https://w3id.org/irnerio-mosaico/ontology/mmdio/> ;
          rdfs:label "ordinary" .


###  https://w3id.org/irnerio/ontology/memo/centimeters
memo:centimeters rdf:type owl:NamedIndividual ,
                          memo:SizeMeasurementUnit ;
                 rdfs:comment "Named individual of size measurement unit. It represents a unit of length or width equal to one hundredth of a meter."@en ;
                 rdfs:isDefinedBy <https://w3id.org/irnerio/ontology/memo> ;
                 rdfs:label "centimeters"@en .


###  https://w3id.org/irnerio/ontology/memo/decimeters
memo:decimeters rdf:type owl:NamedIndividual ,
                         memo:SizeMeasurementUnit ;
                rdfs:comment "Named individual of size measurement unit. It represents a unit of length or width equal to one tenth of a meter."@en ;
                rdfs:isDefinedBy <https://w3id.org/irnerio/ontology/memo> ;
                rdfs:label "decimeters"@en .


###  https://w3id.org/irnerio/ontology/memo/explicit
memo:explicit rdf:type owl:NamedIndividual ,
                       memo:TextualRole ;
              rdfs:comment "A textual role assumed by a textual metadata in time. It is based on the textual string containing the closing words of either the manuscript text, a gloss, or both."@en ;
              rdfs:isDefinedBy <https://w3id.org/irnerio/ontology/memo> ;
              rdfs:label "explicit"@en .


###  https://w3id.org/irnerio/ontology/memo/incipit
memo:incipit rdf:type owl:NamedIndividual ,
                      memo:TextualRole ;
             rdfs:comment "A textual role assumed by a textual metadata in time. It is based on the textual string containing the opening words of either the a manuscript text, a gloss, or both."@en ;
             rdfs:isDefinedBy <https://w3id.org/irnerio/ontology/memo> ;
             rdfs:label "incipit"@en .


###  https://w3id.org/irnerio/ontology/memo/millimeters
memo:millimeters rdf:type owl:NamedIndividual ,
                          memo:SizeMeasurementUnit ;
                 rdfs:comment "Named individual of size measurement unit. It represents a unit of length or width equal to one thousandth of a meter."@en ;
                 rdfs:isDefinedBy <https://w3id.org/irnerio/ontology/memo> ;
                 rdfs:label "millimeters"@en .


###  https://w3id.org/irnerio/ontology/memo/paper
memo:paper rdf:type owl:NamedIndividual ,
                    dcterms:PhysicalMedium ;
           rdfs:comment "Named individual of physical medium. It indicates a thin, flat material made from vegetable fibers."@en ;
           rdfs:isDefinedBy <https://w3id.org/irnerio/ontology/memo> ;
           rdfs:label "paper"@en .


###  https://w3id.org/irnerio/ontology/memo/parchment
memo:parchment rdf:type owl:NamedIndividual ,
                        dcterms:PhysicalMedium ;
               rdfs:comment "Named individual of physical medium. It indicates a material made from animal skin."@en ;
               rdfs:isDefinedBy <https://w3id.org/irnerio/ontology/memo> ;
               rdfs:label "parchment"@en .


###  Generated by the OWL API (version 4.5.26.2023-07-17T20:34:13Z) https://github.com/owlcs/owlapi
